makeHtml.sh
@@ -1,0 +1,3 @@
+eval $(opam env)
+# alectryon -R . Lib -I . --frontend coq proofs.v
+alectryon -R . Lib -I . --frontend coq --backend webpage proofs.v -o html/proofs.html
